make rwlock naming the same as lock naming. regoose pav

src/goose_lang/lib/rwlock/impl.v
@@ -1,42 +1,42 @@
 From Perennial.goose_lang Require Export notation typing.
 
-Module rwlock.
-  Section goose_lang.
-    Context {ext:ffi_syntax}.
+Section goose_lang.
+  Context {ext:ffi_syntax}.
 
-    (* RWlock is a reference call containing a uint 64:
-      - If value is 0, lock is write locked
-      - If value is 1, lock is free
-      - If value is n for n > 1, lock is read locked with (n-1) readers *)
+  (* RWlock is a reference call containing a uint 64:
+    - If value is 0, lock is write locked
+    - If value is 1, lock is free
+    - If value is n for n > 1, lock is read locked with (n-1) readers *)
 
-    Definition new: val := λ: <>, ref #1.
+  Definition newRWMutex : val := λ: <>, ref #1.
 
-    Definition try_read_acquire : val :=
-      λ: "l",
-      let: "n" := ! "l" in
-      if: (#1 ≤ "n") `and` ("n" < "n" + #1) then
-        CAS "l" "n" ("n" + #1)
-      else #false.
+  Definition RWMutex__TryRLock : val :=
+    λ: "l",
+    let: "n" := ! "l" in
+    if: (#1 ≤ "n") `and` ("n" < "n" + #1) then
+      CAS "l" "n" ("n" + #1)
+    else #false.
 
-    Definition read_acquire : val :=
-      rec: "acquire" "l" := if: try_read_acquire "l" then #() else "acquire" "l".
+  Definition RWMutex__RLock : val :=
+    rec: "RWMutex__RLock" "l" := if: RWMutex__TryRLock "l" then #() else "RWMutex__RLock" "l".
 
-    Definition try_read_release : val :=
-      λ: "l",
-      let: "n" := ! "l" in
-      if: (#1 < "n") then
-        CAS "l" "n" ("n" - #1)
-      else #false.
+  (* TODO: RWMutex__TryRUnlock isn't there in actual Golang API. *)
+  Definition RWMutex__TryRUnlock : val :=
+    λ: "l",
+    let: "n" := ! "l" in
+    if: (#1 < "n") then
+      CAS "l" "n" ("n" - #1)
+    else #false.
 
-    Definition read_release : val :=
-      rec: "release" "l" := if: try_read_release "l" then #() else "release" "l".
+  Definition RWMutex__RUnlock : val :=
+    rec: "RWMutex__RUnlock" "l" := if: RWMutex__TryRUnlock "l" then #() else "RWMutex__RUnlock" "l".
 
-    Definition try_write_acquire : val :=
-      λ: "l", CAS "l" #1 #0.
+  Definition RWMutex__TryLock : val :=
+    λ: "l", CAS "l" #1 #0.
 
-    Definition write_acquire : val :=
-      rec: "acquire" "l" := if: try_write_acquire "l" then #() else "acquire" "l".
-    Definition write_release : val := λ: "l", CmpXchg "l" #0 #1;; #().
+  Definition RWMutex__Lock : val :=
+    rec: "RWMutex__Lock" "l" := if: RWMutex__TryLock "l" then #() else "RWMutex__Lock" "l".
 
-  End goose_lang.
-End rwlock.
+  Definition RWMutex__Unlock : val := λ: "l", CmpXchg "l" #0 #1;; #().
+
+End goose_lang.
