src/goose_lang/base_prelude.v
@@ -5,12 +5,10 @@ From Perennial.goose_lang.lib Require Export
      typed_mem.impl struct.impl loop.impl
      encoding.impl map.impl slice.impl lock.impl
      time.impl rand.impl proph.impl waitgroup.impl
-     string.impl atomic.impl
-.
+     string.impl atomic.impl rwlock.impl.
 
 (* We provide stubs here for primitive operations to make the Goose unit tests
    compile. *)
-
 
 Open Scope heap_types.
 Open Scope struct_scope.
